Add LengthDelimited decoder for well-founded uses.

src/Narcissus/Examples/ProtobufLengthDelimited.v
@@ -55,6 +55,11 @@ Section LengthDelimited.
   Variable A_decode_lt : forall b cd x b' cd', A_decode b cd = Some (x, b', cd') -> lt_B b' b.
   Variable A_decode_correct : CorrectDecoder monoid A_predicate A_predicate_rest A_format A_decode A_cache_inv.
 
+  Variable Wf_bound : B.
+  Variable Wf_decode : forall b, lt_B b Wf_bound -> CacheDecode -> option (A * B * CacheDecode).
+  Variable Wf_decode_lt : forall b pf cd x b' cd', Wf_decode b pf cd = Some (x, b', cd') -> lt_B b' b.
+  Variable Wf_decode_correct : CorrectDecoderWf monoid A_predicate A_predicate_rest A_format Wf_decode A_cache_inv.
+
   Definition PB_LengthDelimited_format
     : FormatM (list A) B :=
     (fun xs ce =>
@@ -69,6 +74,18 @@ Section LengthDelimited.
                           Some (N.to_nat x, b1, cd1));
         SizedList_decode A_decode A_decode_lt
                          (sz * 8) b1 cd.
+
+  Definition PB_LengthDelimitedWf_decode
+    : forall b, lt_B b Wf_bound -> CacheDecode -> option (list A * B * CacheDecode).
+  Proof.
+    refine
+      (fun b pf cd =>
+         `(sz, b1, cd1) <- (`(x, b1, cd1) <- Decode_w_Measure_lt Varint_decode b cd Varint_decode_lt;
+                           Some (N.to_nat x, b1, cd1));
+         SizedListWf_decode Wf_bound Wf_decode Wf_decode_lt
+                            (sz * 8) (proj1_sig b1) _ cd).
+    abstract (destruct b1; simpl; unfold lt_B in *; omega).
+  Defined.
 
   Local Arguments Nat.div : simpl never.
   Theorem PB_LengthDelimited_decode_correct
@@ -120,6 +137,55 @@ Section LengthDelimited.
     }
   Qed.
 
+  Theorem PB_LengthDelimitedWf_decode_correct
+          (A_cache_inv_OK : cache_inv_Property A_cache_inv (fun P => forall b cd, P cd -> P (addD cd b)))
+    : CorrectDecoderWf monoid
+                     (fun xs => forall x, In x xs -> A_predicate x)
+                     (SizedList_predicate_rest A_predicate_rest A_format)
+                     PB_LengthDelimited_format PB_LengthDelimitedWf_decode A_cache_inv.
+  Proof.
+    unfold PB_LengthDelimited_format, PB_LengthDelimitedWf_decode.
+    split; intros. {
+      computes_to_inv2.
+      assert (lt_B (mappend b0 ext) Wf_bound) as pf'. {
+        unfold lt_B in *. rewrite !mappend_measure in pf. rewrite mappend_measure. omega.
+      }
+      pose proof (Varint_decode_correct (P:=A_cache_inv)) as Hv.
+      edestruct Hv as [[? [? [? ?]]] _]; eauto. clear H4 H5.
+      edestruct (SizedListWf_decode_correct (A:=A)) as [[? [? [? ?]]] _]; try apply H2; eauto.
+      intuition. eapply SizedList_format_sz_eq; eauto.
+      eexists. repeat split; eauto.
+      edestruct @Decode_w_Measure_lt_eq with (A_decode_lt:=Varint_decode_lt); eauto.
+      revert pf. rewrite <- mappend_assoc. intros. rewrite H7.
+      simpl. rewrite Nat.mul_comm.
+      assert (bin_measure b0 mod 8 = 0) as L. {
+        eapply SizedList_format_byte; eauto.
+      }
+      apply Nat.div_exact in L; eauto. rewrite Nnat.Nat2N.id.
+      rewrite <- L; eauto.
+      match goal with
+      | H : SizedListWf_decode _ _ _ _ _ ?p _ = _ |- 
+        SizedListWf_decode _ _ _ _ _ ?p' _ = _ =>
+        replace p' with p
+      end. apply H4.
+      apply le_uniqueness_proof.
+    } {
+      decode_opt_to_inv.
+      subst. apply Decode_w_Measure_lt_eq_inv in H1. destruct x3. simpl in H1.
+      pose proof (Varint_decode_correct (P:=A_cache_inv)) as Hv.
+      edestruct Hv as [_ [? [? [? [? [? [? ?]]]]]]]; eauto.
+      edestruct (SizedListWf_decode_correct (A:=A)) as [_ [? [? [? [? [? [[? ?] ?]]]]]]]; try apply H2; eauto.
+      split; eauto.
+      eexists _, _. repeat split; eauto.
+      computes_to_econstructor; eauto.
+      computes_to_econstructor; eauto.
+      apply H11 in H9. simpl fst. rewrite H9. rewrite Nat.div_mul by auto. rewrite Nnat.N2Nat.id. eauto.
+      simpl fst. rewrite <- mappend_assoc. subst. simpl in *. congruence.
+    }
+    Grab Existential Variables.
+    auto.
+  Qed.
+
   Theorem PB_LengthDelimited_format_sz_eq
     : forall d b1 b2 ce1 ce1' ce2 ce2',
       PB_LengthDelimited_format d ce1 ↝ (b1, ce1') ->
@@ -143,6 +209,17 @@ Section LengthDelimited.
     decode_opt_to_inv.
     apply Varint_decode_lt in H.
     apply SizedList_decode_le in H0.
+    unfold lt_B, le_B in *. subst. omega.
+  Qed.
+
+  Theorem PB_LengthDelimitedWf_decode_lt
+    : forall b pf cd d b' cd',
+      PB_LengthDelimitedWf_decode b pf cd = Some (d, b', cd') -> lt_B b' b.
+  Proof.
+    unfold PB_LengthDelimited_decode. intros.
+    decode_opt_to_inv.
+    apply Decode_w_Measure_lt_eq_inv in H. destruct x3, x0. simpl in *.
+    apply SizedListWf_decode_le in H0.
     unfold lt_B, le_B in *. subst. omega.
   Qed.
 
